modernized definitions;

thys/RSAPSS/EMSAPSS.thy
@@ -13,168 +13,150 @@ text {* We define the encoding and decoding operations for the probabilistic
  signature scheme. Finally we show, that encoded messages always can be 
  verified *}
 
-consts  BC:: "bv" (* 0xbc *)
-        salt:: "bv"
-        sLen:: "nat" (* length of salt *)
-        generate_M':: "bv \<Rightarrow> bv \<Rightarrow> bv" (* generate_M' outputs "M'" a bit string of length "64 + length(sha1 _ ) + sLen" with 64 initial zero bits *)
-        generate_PS:: "nat \<Rightarrow> nat \<Rightarrow> bv" (* generate_PS outputs "PS" a bit string consisting of "nat (roundup emBits 8) * 8 - sLen - length (sha1 _ ) - 16" zero bits *)
-        generate_DB:: "bv \<Rightarrow> bv" (* generate_DB outputs the bit string DB="PS#(0x01)#salt" of length "nat (roundup emBits 8) * 8 - length (sha1 _ ) - 8" *)
-        generate_H:: "bv \<Rightarrow> nat \<Rightarrow> nat \<Rightarrow> bv" (* generate_H returns a bit string of length (sha1 _) *)
-        generate_maskedDB:: "bv \<Rightarrow> nat \<Rightarrow> nat \<Rightarrow> bv " (* outputs a bit string of length "nat (roundup emBits 8) * 8 - length (sha1 _) - 8" *)
-        generate_salt:: "bv \<Rightarrow> bv" (* outputs a bit string of length sLen *)
-        show_rightmost_bits:: "bv \<Rightarrow> nat \<Rightarrow> bv" (* extract n rightmost bits of a bit string*)
-        MGF:: "bv \<Rightarrow> nat \<Rightarrow> bv" (* mask generation function *)
-        MGF1:: "bv \<Rightarrow> nat \<Rightarrow> nat \<Rightarrow> bv" (* help function for MGF *)
-        maskedDB_zero:: "bv \<Rightarrow> nat \<Rightarrow> bv" (* sets "roundup emBits 8 * 8 - emBits" bits of maskedDB to zero *)
-        emsapss_encode:: "bv \<Rightarrow> nat \<Rightarrow> bv" (* outputs the encoded message of length emBits *)
-        emsapss_encode_help1:: "bv \<Rightarrow> nat \<Rightarrow> bv"
-        emsapss_encode_help2:: "bv \<Rightarrow> nat \<Rightarrow> bv"
-        emsapss_encode_help3:: "bv \<Rightarrow> nat \<Rightarrow> bv"
-        emsapss_encode_help4:: "bv \<Rightarrow> bv \<Rightarrow> nat \<Rightarrow> bv"
-        emsapss_encode_help5:: "bv \<Rightarrow> bv \<Rightarrow> nat \<Rightarrow> bv"
-        emsapss_encode_help6:: "bv \<Rightarrow> bv \<Rightarrow> bv \<Rightarrow> nat \<Rightarrow> bv"
-        emsapss_encode_help7:: "bv \<Rightarrow> bv \<Rightarrow> nat \<Rightarrow> bv"
-        emsapss_encode_help8:: "bv \<Rightarrow> bv \<Rightarrow> bv"
-        emsapss_decode:: "bv \<Rightarrow> bv \<Rightarrow> nat \<Rightarrow> bool" (* outputs "true" if EM is encoding of M *)
-        emsapss_decode_help1:: "bv \<Rightarrow> bv \<Rightarrow> nat \<Rightarrow> bool"
-        emsapss_decode_help2:: "bv \<Rightarrow> bv \<Rightarrow> nat \<Rightarrow> bool"
-        emsapss_decode_help3:: "bv \<Rightarrow> bv \<Rightarrow> nat \<Rightarrow> bool"
-        emsapss_decode_help4:: "bv \<Rightarrow> bv \<Rightarrow> bv \<Rightarrow> nat \<Rightarrow> bool"
-        emsapss_decode_help5:: "bv \<Rightarrow> bv \<Rightarrow> bv \<Rightarrow> bv \<Rightarrow> nat \<Rightarrow> bool"
-        emsapss_decode_help6:: "bv \<Rightarrow> bv \<Rightarrow> bv \<Rightarrow> nat \<Rightarrow> bool"
-        emsapss_decode_help7:: "bv \<Rightarrow> bv \<Rightarrow> bv \<Rightarrow> nat \<Rightarrow> bool"
-        emsapss_decode_help8:: "bv \<Rightarrow> bv \<Rightarrow> bv \<Rightarrow> bool"
-        emsapss_decode_help9:: "bv \<Rightarrow> bv \<Rightarrow> bv \<Rightarrow> bool"
-        emsapss_decode_help10:: "bv \<Rightarrow> bv \<Rightarrow> bool"
-        emsapss_decode_help11:: "bv \<Rightarrow> bv \<Rightarrow> bool"
+definition show_rightmost_bits:: "bv \<Rightarrow> nat \<Rightarrow> bv" (* extract n rightmost bits of a bit string*)
+  where "show_rightmost_bits bvec n = rev (take n (rev bvec))"
 
-defs
+definition BC:: "bv" (* 0xbc *)
+  where "BC = [One, Zero, One, One, One, One, Zero, Zero]"
 
-  show_rightmost_bits:
-  "show_rightmost_bits bvec n == rev(take n (rev bvec) )"
+definition salt:: "bv"
+  where "salt = []"
 
-  BC:
-  "BC == [One, Zero, One, One, One, One, Zero, Zero]"
+definition sLen:: "nat" (* length of salt *)
+  where "sLen = length salt"
 
-  salt:
-  "salt  == []"
+definition generate_M':: "bv \<Rightarrow> bv \<Rightarrow> bv" (* generate_M' outputs "M'" a bit string of length "64 + length(sha1 _ ) + sLen" with 64 initial zero bits *)
+  where "generate_M' mHash salt_new = bv_prepend 64 \<zero> [] @ mHash @ salt_new"
 
-  sLen:
-  "sLen == length salt"
+definition generate_PS:: "nat \<Rightarrow> nat \<Rightarrow> bv" (* generate_PS outputs "PS" a bit string consisting of "nat (roundup emBits 8) * 8 - sLen - length (sha1 _ ) - 16" zero bits *)
+  where "generate_PS emBits hLen = bv_prepend ((roundup emBits 8)*8 - sLen - hLen - 16) \<zero> []"
 
-  generate_M':
-  "generate_M' mHash salt_new  == (bv_prepend 64 \<zero> []) @ mHash @ salt_new"
+definition generate_DB:: "bv \<Rightarrow> bv" (* generate_DB outputs the bit string DB="PS#(0x01)#salt" of length "nat (roundup emBits 8) * 8 - length (sha1 _ ) - 8" *)
+  where "generate_DB PS = PS @ [Zero, Zero, Zero, Zero, Zero, Zero, Zero, One] @ salt"
 
-  generate_PS:
-  "generate_PS emBits hLen == bv_prepend ((roundup emBits 8)*8 - sLen - hLen - 16) \<zero> []"
+definition maskedDB_zero:: "bv \<Rightarrow> nat \<Rightarrow> bv" (* sets "roundup emBits 8 * 8 - emBits" bits of maskedDB to zero *)
+  where "maskedDB_zero maskedDB emBits = bv_prepend ((roundup emBits 8) * 8 - emBits)  \<zero> (drop ((roundup emBits 8)*8 - emBits) maskedDB)"
 
-  generate_DB:
-  "generate_DB PS == PS @ [Zero, Zero, Zero, Zero, Zero, Zero, Zero, One] @ salt"
+definition generate_H:: "bv \<Rightarrow> nat \<Rightarrow> nat \<Rightarrow> bv" (* generate_H returns a bit string of length (sha1 _) *)
+  where "generate_H EM emBits hLen = take hLen (drop ((roundup emBits 8)*8 - hLen - 8) EM)"
 
-  maskedDB_zero:
-  "maskedDB_zero maskedDB emBits == bv_prepend ((roundup emBits 8) * 8 - emBits)  \<zero> (drop ((roundup emBits 8)*8 - emBits) maskedDB)"
+definition generate_maskedDB:: "bv \<Rightarrow> nat \<Rightarrow> nat \<Rightarrow> bv " (* outputs a bit string of length "nat (roundup emBits 8) * 8 - length (sha1 _) - 8" *)
+  where "generate_maskedDB EM emBits hLen = take ((roundup emBits 8)*8 - hLen - 8) EM"
 
-  generate_H:
-  "generate_H EM emBits hLen == take hLen (drop ((roundup emBits 8)*8 - hLen - 8) EM)"
+definition generate_salt:: "bv \<Rightarrow> bv" (* outputs a bit string of length sLen *)
+  where "generate_salt DB_zero = show_rightmost_bits DB_zero sLen"
 
-  generate_maskedDB:
-  "generate_maskedDB EM emBits hLen == take ((roundup emBits 8)*8 - hLen - 8) EM"
-
-  generate_salt:
-  "generate_salt DB_zero == show_rightmost_bits DB_zero sLen"
-
-primrec MGF2:: "bv \<Rightarrow> nat \<Rightarrow> bv" (* help function for MGF1 *) where
+primrec MGF2:: "bv \<Rightarrow> nat \<Rightarrow> bv" (* help function for MGF1 *)
+where
   "MGF2 Z 0 = sha1 (Z@(nat_to_bv_length 0 32))"
 | "MGF2 Z (Suc n) = (MGF2 Z n)@(sha1 (Z@(nat_to_bv_length (Suc n) 32)))"
 
-defs
-  MGF:
-  "MGF Z l == if l = 0 \<or> 2^32*(length (sha1 Z)) < l
+definition MGF1:: "bv \<Rightarrow> nat \<Rightarrow> nat \<Rightarrow> bv" (* help function for MGF *)
+  where "MGF1 Z n l = take l (MGF2 Z n)"
+
+definition MGF:: "bv \<Rightarrow> nat \<Rightarrow> bv" (* mask generation function *)
+where
+  "MGF Z l = (if l = 0 \<or> 2^32*(length (sha1 Z)) < l
               then []
-              else MGF1 Z ( roundup l (length (sha1 Z))  - 1 ) l"
+              else MGF1 Z ( roundup l (length (sha1 Z))  - 1 ) l)"
 
-  MGF1:
-  "MGF1 Z n l== take l (MGF2 Z n)"
 
-  emsapss_encode:
-  "emsapss_encode M emBits == if (2^64 \<le> length M \<or> 2^32 * 160 < emBits)
-                              then []
-                              else emsapss_encode_help1 (sha1 M) emBits"
+definition emsapss_encode_help8:: "bv \<Rightarrow> bv \<Rightarrow> bv"
+  where "emsapss_encode_help8 DBzero H = DBzero @ H @ BC"
 
-  emsapss_encode_help1:
-  "emsapss_encode_help1 mHash emBits == if emBits  < length (mHash) + sLen + 16
-                                        then []
-                                        else emsapss_encode_help2 (generate_M' mHash salt) emBits"
-  emsapss_encode_help2:
-  "emsapss_encode_help2 M' emBits == emsapss_encode_help3 (sha1 M') emBits"
+definition emsapss_encode_help7:: "bv \<Rightarrow> bv \<Rightarrow> nat \<Rightarrow> bv"
+  where "emsapss_encode_help7 maskedDB H emBits =
+    emsapss_encode_help8 (maskedDB_zero maskedDB emBits) H"
 
-  emsapss_encode_help3:
-  "emsapss_encode_help3 H emBits == emsapss_encode_help4 (generate_PS emBits (length H)) H emBits"
+definition emsapss_encode_help6:: "bv \<Rightarrow> bv \<Rightarrow> bv \<Rightarrow> nat \<Rightarrow> bv"
+  where "emsapss_encode_help6 DB dbMask H emBits =
+    (if dbMask = []
+     then []
+     else emsapss_encode_help7 (bvxor DB dbMask) H emBits)"
 
-  emsapss_encode_help4:
-  "emsapss_encode_help4 PS H emBits == emsapss_encode_help5 (generate_DB PS) H emBits"
+definition emsapss_encode_help5:: "bv \<Rightarrow> bv \<Rightarrow> nat \<Rightarrow> bv"
+  where "emsapss_encode_help5 DB H emBits =
+    emsapss_encode_help6 DB (MGF H (length DB)) H emBits"
 
-  emsapss_encode_help5:
-  "emsapss_encode_help5 DB H emBits == emsapss_encode_help6 DB (MGF H (length DB)) H emBits"
+definition emsapss_encode_help4:: "bv \<Rightarrow> bv \<Rightarrow> nat \<Rightarrow> bv"
+  where "emsapss_encode_help4 PS H emBits =
+    emsapss_encode_help5 (generate_DB PS) H emBits"
 
-  emsapss_encode_help6:
-  "emsapss_encode_help6 DB dbMask H emBits == if dbMask = []
-                                              then []
-                                              else emsapss_encode_help7 (bvxor DB dbMask) H emBits"
+definition emsapss_encode_help3:: "bv \<Rightarrow> nat \<Rightarrow> bv"
+  where "emsapss_encode_help3 H emBits =
+    emsapss_encode_help4 (generate_PS emBits (length H)) H emBits"
 
-  emsapss_encode_help7:
-  "emsapss_encode_help7 maskedDB H emBits == emsapss_encode_help8 (maskedDB_zero maskedDB emBits) H"
+definition emsapss_encode_help2:: "bv \<Rightarrow> nat \<Rightarrow> bv"
+  where "emsapss_encode_help2 M' emBits = emsapss_encode_help3 (sha1 M') emBits"
 
-  emsapss_encode_help8:
-  "emsapss_encode_help8 DBzero H == DBzero @ H @ BC"
+definition emsapss_encode_help1:: "bv \<Rightarrow> nat \<Rightarrow> bv"
+  where "emsapss_encode_help1 mHash emBits =
+    (if emBits  < length (mHash) + sLen + 16
+     then []
+     else emsapss_encode_help2 (generate_M' mHash salt) emBits)"
 
-  emsapss_decode:
-  "emsapss_decode M EM emBits == if (2^64 \<le> length M \<or> 2^32*160<emBits)
-                                 then False
-                                 else emsapss_decode_help1 (sha1 M) EM emBits"
+definition emsapss_encode:: "bv \<Rightarrow> nat \<Rightarrow> bv" (* outputs the encoded message of length emBits *)
+  where "emsapss_encode M emBits =
+    (if (2^64 \<le> length M \<or> 2^32 * 160 < emBits)
+     then []
+     else emsapss_encode_help1 (sha1 M) emBits)"
 
-  emsapss_decode_help1:
-  "emsapss_decode_help1 mHash EM emBits == if emBits < length (mHash) + sLen + 16
-                                           then False 
-                                           else emsapss_decode_help2 mHash EM emBits"
 
-  emsapss_decode_help2:
-  "emsapss_decode_help2 mHash EM emBits == if show_rightmost_bits EM 8 \<noteq> BC
-                                           then False
-                                           else emsapss_decode_help3 mHash EM emBits"
+definition emsapss_decode_help11:: "bv \<Rightarrow> bv \<Rightarrow> bool"
+  where "emsapss_decode_help11 H' H = (if H' \<noteq> H then False else True)"
 
-  emsapss_decode_help3:
-  "emsapss_decode_help3 mHash EM emBits == emsapss_decode_help4 mHash (generate_maskedDB EM emBits (length mHash)) (generate_H EM emBits (length mHash)) emBits"
+definition emsapss_decode_help10:: "bv \<Rightarrow> bv \<Rightarrow> bool"
+  where "emsapss_decode_help10 M' H = emsapss_decode_help11 (sha1 M') H"
 
-  emsapss_decode_help4:
-  "emsapss_decode_help4 mHash maskedDB H emBits == if take ((roundup emBits 8)*8 - emBits) maskedDB \<noteq> bv_prepend ((roundup emBits 8)*8 - emBits) \<zero> []
-                                                   then False
-                                                   else emsapss_decode_help5 mHash maskedDB (MGF H ((roundup emBits 8)*8 - (length mHash) - 8)) H emBits"
+definition emsapss_decode_help9:: "bv \<Rightarrow> bv \<Rightarrow> bv \<Rightarrow> bool"
+  where "emsapss_decode_help9 mHash salt_new H =
+    emsapss_decode_help10 (generate_M' mHash salt_new) H"
 
-  emsapss_decode_help5:
-  "emsapss_decode_help5 mHash maskedDB dbMask H emBits == emsapss_decode_help6 mHash (bvxor maskedDB dbMask) H emBits"
+definition emsapss_decode_help8:: "bv \<Rightarrow> bv \<Rightarrow> bv \<Rightarrow> bool"
+  where "emsapss_decode_help8 mHash DB_zero H =
+    emsapss_decode_help9 mHash (generate_salt DB_zero) H"
 
-  emsapss_decode_help6:
-  "emsapss_decode_help6 mHash DB H emBits == emsapss_decode_help7 mHash (maskedDB_zero DB emBits) H emBits"
+definition emsapss_decode_help7:: "bv \<Rightarrow> bv \<Rightarrow> bv \<Rightarrow> nat \<Rightarrow> bool"
+  where "emsapss_decode_help7 mHash DB_zero H emBits =
+   (if (take ( (roundup emBits 8)*8 - (length mHash) - sLen - 16) DB_zero \<noteq> bv_prepend ( (roundup emBits 8)*8 - (length mHash) - sLen - 16) \<zero> []) \<or> (take 8 ( drop ((roundup emBits 8)*8 - (length mHash) - sLen - 16 ) DB_zero ) \<noteq> [Zero, Zero, Zero, Zero, Zero, Zero, Zero, One])
+    then False
+    else emsapss_decode_help8 mHash DB_zero H)"
 
-  emsapss_decode_help7:
-  "emsapss_decode_help7 mHash DB_zero H emBits == if (take ( (roundup emBits 8)*8 - (length mHash) - sLen - 16) DB_zero \<noteq> bv_prepend ( (roundup emBits 8)*8 - (length mHash) - sLen - 16) \<zero> []) \<or> (take 8 ( drop ((roundup emBits 8)*8 - (length mHash) - sLen - 16 ) DB_zero ) \<noteq> [Zero, Zero, Zero, Zero, Zero, Zero, Zero, One])
-                                                  then False
-                                                  else emsapss_decode_help8 mHash DB_zero H"
+definition emsapss_decode_help6:: "bv \<Rightarrow> bv \<Rightarrow> bv \<Rightarrow> nat \<Rightarrow> bool"
+  where "emsapss_decode_help6 mHash DB H emBits =
+    emsapss_decode_help7 mHash (maskedDB_zero DB emBits) H emBits"
 
-  emsapss_decode_help8:
-  "emsapss_decode_help8 mHash DB_zero H == emsapss_decode_help9 mHash (generate_salt DB_zero) H"
+definition emsapss_decode_help5:: "bv \<Rightarrow> bv \<Rightarrow> bv \<Rightarrow> bv \<Rightarrow> nat \<Rightarrow> bool"
+  where "emsapss_decode_help5 mHash maskedDB dbMask H emBits =
+    emsapss_decode_help6 mHash (bvxor maskedDB dbMask) H emBits"
 
-  emsapss_decode_help9:
-  "emsapss_decode_help9 mHash salt_new H == emsapss_decode_help10 (generate_M' mHash salt_new) H"
+definition emsapss_decode_help4:: "bv \<Rightarrow> bv \<Rightarrow> bv \<Rightarrow> nat \<Rightarrow> bool"
+  where "emsapss_decode_help4 mHash maskedDB H emBits =
+   (if take ((roundup emBits 8)*8 - emBits) maskedDB \<noteq> bv_prepend ((roundup emBits 8)*8 - emBits) \<zero> []
+    then False
+    else emsapss_decode_help5 mHash maskedDB (MGF H ((roundup emBits 8)*8 - (length mHash) - 8)) H emBits)"
 
-  emsapss_decode_help10:
-  "emsapss_decode_help10 M' H == emsapss_decode_help11 (sha1 M') H"
+definition emsapss_decode_help3:: "bv \<Rightarrow> bv \<Rightarrow> nat \<Rightarrow> bool"
+  where "emsapss_decode_help3 mHash EM emBits =
+    emsapss_decode_help4 mHash (generate_maskedDB EM emBits (length mHash)) (generate_H EM emBits (length mHash)) emBits"
 
-  emsapss_decode_help11:
-  "emsapss_decode_help11 H' H == if H' \<noteq> H
-                                 then False
-                                 else True"
+definition emsapss_decode_help2:: "bv \<Rightarrow> bv \<Rightarrow> nat \<Rightarrow> bool"
+  where "emsapss_decode_help2 mHash EM emBits =
+   (if show_rightmost_bits EM 8 \<noteq> BC
+    then False
+    else emsapss_decode_help3 mHash EM emBits)"
+
+definition emsapss_decode_help1:: "bv \<Rightarrow> bv \<Rightarrow> nat \<Rightarrow> bool"
+  where "emsapss_decode_help1 mHash EM emBits =
+    (if emBits < length (mHash) + sLen + 16
+     then False 
+     else emsapss_decode_help2 mHash EM emBits)"
+
+definition emsapss_decode:: "bv \<Rightarrow> bv \<Rightarrow> nat \<Rightarrow> bool" (* outputs "true" if EM is encoding of M *)
+  where "emsapss_decode M EM emBits =
+    (if (2^64 \<le> length M \<or> 2^32*160<emBits)
+     then False
+     else emsapss_decode_help1 (sha1 M) EM emBits)"
 
 lemma roundup_positiv: "0 < emBits \<Longrightarrow> 0 < (roundup emBits 160)"
   by (simp add: roundup, safe, simp)
@@ -202,7 +184,7 @@ lemma roundup_le_7: "0 < emBits \<Longrightarrow> roundup emBits 8 * 8 - emBits 
 lemma roundup_nat_ge_8_help:
   "length (sha1 M) + sLen + 16 \<le> emBits \<Longrightarrow> 8 \<le> roundup emBits 8 * 8 - (length (sha1 M) + 8)"
   apply (insert roundup_ge_emBits [of emBits 8])
-  apply (simp add: roundup sha1len sLen)
+  apply (simp add: roundup sha1len sLen_def)
   done
 
 lemma roundup_nat_ge_8:
@@ -234,7 +216,7 @@ lemma roundup_help1_new: "\<lbrakk> 0 < l\<rbrakk> \<Longrightarrow> (roundup l 
   done
 
 lemma roundup_help2: "\<lbrakk>176 + sLen \<le> emBits\<rbrakk> \<Longrightarrow> roundup emBits 8 * 8 - emBits <=  roundup emBits 8 * 8 - 160 - sLen - 16"
-  by (simp add: sLen)
+  by (simp add: sLen_def)
 
 lemma bv_prepend_equal: "bv_prepend (Suc n) b l = b#bv_prepend n b l" 
   by (simp add: bv_prepend)
@@ -281,10 +263,10 @@ lemma bv_prepend_split: "bv_prepend x b (left @ right) = bv_prepend x b left @ r
   by (induct x) (simp add: bv_prepend)+
 
 lemma length_generate_DB: "length (generate_DB PS) = length PS + 8 + sLen"
-  by (simp add: generate_DB sLen)
+  by (simp add: generate_DB_def sLen_def)
 
 lemma length_generate_PS: "length (generate_PS emBits 160) = (roundup emBits 8)*8 - sLen - 160 - 16"
-  by (simp add: generate_PS length_bv_prepend)
+  by (simp add: generate_PS_def length_bv_prepend)
 
 lemma length_bvxor: "length a = length b \<Longrightarrow> length (bvxor a b) = length a"
   by (simp add: bvxor)
@@ -293,10 +275,10 @@ lemma length_MGF2: "length (MGF2 Z m) = Suc m * length (sha1 (Z @ nat_to_bv_leng
   by (induct m) (simp+, simp add: sha1len)
 
 lemma length_MGF1: "l \<le> (Suc n) * 160 \<Longrightarrow> length (MGF1 Z n l) = l"
-  by (simp add: MGF1 length_MGF2 sha1len)
+  by (simp add: MGF1_def length_MGF2 sha1len)
 
 lemma length_MGF: "0 < l \<Longrightarrow> l \<le>  2^32 * length (sha1 x) \<Longrightarrow> length (MGF x l) = l"
-  apply (simp add: MGF sha1len)
+  apply (simp add: MGF_def sha1len)
   apply (insert roundup_help1_new [of l])
   apply (rule length_MGF1)
   apply (simp)
@@ -314,18 +296,19 @@ lemma solve_length_generate_DB:
 lemma length_maskedDB_zero:
   "\<lbrakk> roundup emBits 8 * 8 - emBits \<le> length maskedDB\<rbrakk>
   \<Longrightarrow> length (maskedDB_zero maskedDB emBits) = length maskedDB"
-  by (simp add: maskedDB_zero length_bv_prepend)
+  by (simp add: maskedDB_zero_def length_bv_prepend)
 
 lemma take_equal_bv_prepend:
   "\<lbrakk> 176 + sLen \<le> emBits; roundup emBits 8 * 8 - emBits \<le> 7\<rbrakk>
   \<Longrightarrow> take (roundup emBits 8 * 8 - length (sha1 M) - sLen - 16) (maskedDB_zero (generate_DB (generate_PS emBits 160)) emBits) =
     bv_prepend (roundup emBits 8 * 8 - length (sha1 M) - sLen - 16) \<zero> []"
   apply (insert roundup_help2 [of emBits] length_generate_PS [of emBits])
-  apply (simp add: sha1len maskedDB_zero generate_DB generate_PS bv_prepend_split bv_prepend_drop)
+  apply (simp add: sha1len maskedDB_zero_def generate_DB_def generate_PS_def
+    bv_prepend_split bv_prepend_drop)
   done
 
 lemma lastbits_BC: "BC = show_rightmost_bits (xs @ ys @ BC) 8"
-  by (simp add:show_rightmost_bits BC)
+  by (simp add: show_rightmost_bits_def BC_def)
 
 lemma equal_zero:
   "176 + sLen \<le> emBits \<Longrightarrow> roundup emBits 8 * 8 - emBits \<le> roundup emBits 8 * 8 - (176 + sLen)
@@ -334,20 +317,21 @@ lemma equal_zero:
 
 lemma get_salt: "\<lbrakk> 176 + sLen \<le> emBits; roundup emBits 8 * 8 - emBits \<le> 7\<rbrakk> \<Longrightarrow> (generate_salt (maskedDB_zero (generate_DB (generate_PS emBits 160)) emBits)) = salt"
   apply (insert roundup_help2 [of emBits] length_generate_PS [of emBits] equal_zero [of emBits])
-  apply (simp add: generate_DB generate_PS maskedDB_zero)
-  apply (simp add: bv_prepend_split bv_prepend_drop generate_salt show_rightmost_bits sLen)
+  apply (simp add: generate_DB_def generate_PS_def maskedDB_zero_def)
+  apply (simp add: bv_prepend_split bv_prepend_drop generate_salt_def
+    show_rightmost_bits_def sLen_def)
   done
 
 lemma generate_maskedDB_elim: "\<lbrakk>roundup emBits 8 * 8 - emBits \<le> length x; ( roundup emBits 8) * 8 - (length (sha1 M)) - 8 = length (maskedDB_zero x emBits)\<rbrakk> \<Longrightarrow> generate_maskedDB (maskedDB_zero x emBits @ y @ z) emBits (length(sha1 M)) = maskedDB_zero x emBits"
-  apply (simp add: maskedDB_zero)
+  apply (simp add: maskedDB_zero_def)
   apply (insert length_bv_prepend_drop [of "(roundup emBits 8 * 8 - emBits)" "x"])
-  apply (simp add: generate_maskedDB)
+  apply (simp add: generate_maskedDB_def)
   done
 
 lemma generate_H_elim: "\<lbrakk> roundup emBits 8 * 8 - emBits \<le> length x; length (maskedDB_zero x emBits) =  (roundup emBits 8) * 8 - 168; length y = 160\<rbrakk> \<Longrightarrow> generate_H (maskedDB_zero x emBits @ y @ z) emBits 160 = y"
-  apply (simp add: maskedDB_zero)
+  apply (simp add: maskedDB_zero_def)
   apply (insert length_bv_prepend_drop [of "roundup emBits 8 * 8 - emBits" "x"])
-  apply (simp add: generate_H)
+  apply (simp add: generate_H_def)
   done
 
 lemma length_bv_prepend_drop_special: "[|roundup emBits 8 * 8 - emBits <= roundup emBits 8 * 8 - (176 + sLen); length (generate_PS emBits 160) = roundup emBits 8 * 8 - (176 + sLen)|] ==> length ( bv_prepend (roundup emBits 8 * 8 - emBits) \<zero> (drop (roundup emBits 8 * 8 - emBits) (generate_PS emBits 160))) = length (generate_PS emBits 160)"
@@ -355,7 +339,8 @@ lemma length_bv_prepend_drop_special: "[|roundup emBits 8 * 8 - emBits <= roundu
 
 lemma x01_elim: "\<lbrakk>176 + sLen \<le> emBits; roundup emBits 8 * 8 - emBits \<le> 7\<rbrakk> \<Longrightarrow> take 8 (drop (roundup emBits 8 * 8 - (length (sha1 M) + sLen + 16))(maskedDB_zero (generate_DB (generate_PS emBits 160)) emBits)) = [\<zero>, \<zero>, \<zero>, \<zero>, \<zero>, \<zero>, \<zero>, \<one>]"
   apply (insert roundup_help2 [of emBits] length_generate_PS [of emBits] equal_zero [of emBits])
-  apply (simp add: sha1len maskedDB_zero generate_DB generate_PS bv_prepend_split bv_prepend_drop)
+  apply (simp add: sha1len maskedDB_zero_def generate_DB_def generate_PS_def
+    bv_prepend_split bv_prepend_drop)
   done
 
 lemma drop_bv_mapzip:
@@ -415,46 +400,48 @@ proof -
 qed
 
 lemma bvxorxor_elim: "\<lbrakk> roundup emBits 8 * 8 - emBits \<le> length a; length a = length b\<rbrakk> \<Longrightarrow> (maskedDB_zero (bvxor (maskedDB_zero (bvxor a b) emBits)b) emBits) = bv_prepend (roundup emBits 8 * 8 - emBits) \<zero> (drop (roundup emBits 8 * 8 - emBits) a)"
-  by (simp add: maskedDB_zero bvxorxor_elim_help)
+  by (simp add: maskedDB_zero_def bvxorxor_elim_help)
 
 lemma verify: "\<lbrakk>(emsapss_encode M emBits) \<noteq> []; EM=(emsapss_encode M emBits)\<rbrakk> \<Longrightarrow> emsapss_decode M EM emBits = True"
-  apply (simp add: emsapss_decode emsapss_encode)
+  apply (simp add: emsapss_decode_def emsapss_encode_def)
   apply (safe, simp+)
-  apply (simp add: emsapss_decode_help1 emsapss_encode_help1)
+  apply (simp add: emsapss_decode_help1_def emsapss_encode_help1_def)
   apply (safe, simp+)
-  apply (simp add: emsapss_decode_help2 emsapss_encode_help2)
+  apply (simp add: emsapss_decode_help2_def emsapss_encode_help2_def)
   apply (safe)
-  apply (simp add: emsapss_encode_help3 emsapss_encode_help4 emsapss_encode_help5 emsapss_encode_help6)
+  apply (simp add: emsapss_encode_help3_def emsapss_encode_help4_def
+    emsapss_encode_help5_def emsapss_encode_help6_def)
   apply (safe)
-  apply (simp add: emsapss_encode_help7 emsapss_encode_help8 lastbits_BC [symmetric])+
-  apply (simp add: emsapss_decode_help3 emsapss_encode_help3 emsapss_decode_help4 emsapss_encode_help4)
+  apply (simp add: emsapss_encode_help7_def emsapss_encode_help8_def lastbits_BC [symmetric])+
+  apply (simp add: emsapss_decode_help3_def emsapss_encode_help3_def
+    emsapss_decode_help4_def emsapss_encode_help4_def)
   apply (safe)
   apply (insert roundup_le_7 [of emBits] roundup_ge_0 [of emBits 8] roundup_nat_ge_8 [of M emBits])
-  apply (simp add: generate_maskedDB emsapss_encode_help5 emsapss_encode_help6)
+  apply (simp add: generate_maskedDB_def emsapss_encode_help5_def emsapss_encode_help6_def)
   apply (safe)
   apply (simp)
-  apply (simp add: emsapss_encode_help7)
-  apply (simp only: emsapss_encode_help8)
-  apply (simp only: maskedDB_zero)
+  apply (simp add: emsapss_encode_help7_def)
+  apply (simp only: emsapss_encode_help8_def)
+  apply (simp only: maskedDB_zero_def)
   apply (simp only: take_bv_prepend2 min.absorb1)
   apply (simp)
-  apply (simp add: emsapss_encode_help5 emsapss_encode_help6)
+  apply (simp add: emsapss_encode_help5_def emsapss_encode_help6_def)
   apply (safe)
   apply (simp)+
   apply (insert solve_length_generate_DB [of emBits M "generate_M' (sha1 M) salt"] roundup_le_ub [of emBits])
   apply (insert length_MGF [of "(roundup emBits 8) * 8 - 168" "(sha1 (generate_M' (sha1 M) salt))"])
   apply (insert modify_roundup_ge1 [of emBits] modify_roundup_ge2 [of emBits])
-  apply (simp add: sha1len emsapss_encode_help7 emsapss_encode_help8)
+  apply (simp add: sha1len emsapss_encode_help7_def emsapss_encode_help8_def)
   apply (insert length_bvxor [of "(generate_DB (generate_PS emBits 160))" "(MGF (sha1 (generate_M' (sha1 M) salt)) ((roundup emBits 8) * 8 - 168))"])
   apply (insert generate_maskedDB_elim [of emBits "(bvxor (generate_DB (generate_PS emBits 160))(MGF (sha1 (generate_M' (sha1 M) salt)) ((roundup emBits 8) * 8 - 168)))" M "sha1 (generate_M' (sha1 M) salt)" BC])
   apply (insert length_maskedDB_zero [of emBits "(bvxor (generate_DB (generate_PS emBits 160))(MGF (sha1 (generate_M' (sha1 M) salt)) ((roundup emBits 8) * 8 - 168)))"])
   apply (insert generate_H_elim [of emBits "(bvxor (generate_DB (generate_PS emBits 160))(MGF (sha1 (generate_M' (sha1 M) salt)) (roundup emBits 8 * 8 - 168)))" "sha1 (generate_M' (sha1 M) salt)" BC])
-  apply (simp add: sha1len emsapss_decode_help5)
-  apply (simp only: emsapss_decode_help6 emsapss_decode_help7)
+  apply (simp add: sha1len emsapss_decode_help5_def)
+  apply (simp only: emsapss_decode_help6_def emsapss_decode_help7_def)
   apply (insert bvxorxor_elim [of emBits "(generate_DB (generate_PS emBits 160))" "(MGF (sha1 (generate_M' (sha1 M) salt)) ((roundup emBits 8) * 8 - 168))"])
-  apply (fold maskedDB_zero)
+  apply (fold maskedDB_zero_def)
   apply (insert take_equal_bv_prepend [of emBits M] x01_elim [of emBits M] get_salt [of emBits])
-  apply (simp add: emsapss_decode_help8 emsapss_decode_help9 emsapss_decode_help10 emsapss_decode_help11) 
+  apply (simp add: emsapss_decode_help8_def emsapss_decode_help9_def emsapss_decode_help10_def emsapss_decode_help11_def) 
   done
 
 end
